sin module

examples/L1Cache.v
@@ -62,7 +62,7 @@ Section L1Cache.
   End UtilFunctions.
 
   Definition l1Cache :=
-    META {
+    SIN {
         Register "procRqValid": Bool <- @ConstBool false
         with Register "procRq": RqFromProc <- Default
         with Register "procRqReplace": Bool <- @ConstBool false
@@ -252,9 +252,10 @@ Section Facts.
   Variables IdxBits TagBits LgNumDatas LgDataBytes: nat.
   Variable Id: Kind.
 
-  Lemma l1Cache_ModEquiv:
+  Lemma l1Cache_ModEquiv n:
     forall m,
-      m = ParametricSyntax.makeModule (l1Cache IdxBits TagBits LgNumDatas LgDataBytes Id) ->
+      m = ParametricSyntax.makeModule
+            (getMetaFromSinNat n (l1Cache IdxBits TagBits LgNumDatas LgDataBytes Id)) ->
       (forall ty1 ty2, ModEquiv ty1 ty2 m).
   Proof. (* SKIP_PROOF_ON
     kequiv.
@@ -263,5 +264,7 @@ Section Facts.
 
 End Facts.
 
+
 Hint Resolve l1Cache_ModEquiv.
+
 
